---
dg-publish: true
---
#Notes 

Consider a source that emits quantum states at random. For example, the source might be a person, who tosses a biased coin, and depending on the outcome, then emits 

$$
\text{Heads} \to |0\rangle\qquad \text{Tails} \to |+\rangle
$$

Let's imagine the coin is biased in such a way that $P(\text{Heads})=\frac{1}{4}$ and $P(\text{Tails})=\frac{3}{4}$. How can we characterise the properties of this system? We will soon see that to do this, we use **density operator formalism**.

Consider measuring the operator $Z=|0\rangle \langle 0|-|1\rangle \langle 1|$ on the emitted system. The probability to obtain the outcome +1 is just the *average* probability to do so. We can use the **total law of probability** to say the the probability of this outcome is.

$$
P(\text{Event}) = P(\text{Event} | A) \cdot P(A) + P(\text{Event}|B)\cdot P(B)
$$

for two *mutually exclusive* events $A$ and $B$. 

Hence, for our system:

$$
\begin{align}
P(+1)&=P(\text{state is }|0\rangle ) \cdot P(+1 | \text{state is }|0\rangle )+P(\text{state is }|+\rangle ) \cdot P(+1|\text{state is }|+\rangle ) 
\end{align}
	$$

We know $P(\text{state is }|0\rangle)=\frac{1}{4}$ and $P(\text{state is }|+\rangle)=\frac{3}{4}$.

If we get the outcome +1, that means we measured $|0\rangle \langle 0|$ in $Z$, and so our projector of relevance here is $\Pi_{+1}=|0\rangle \langle {0}|$. Hence, the conditional probabilities are 

$$
\begin{align}
P(+1 | \text{state is }|0\rangle )&=|| \Pi_{+1} |0\rangle ||^2 =||(|0\rangle \langle  0|)|0\rangle ||^{2}=|||0\rangle \langle 0|0\rangle ||^2\\ \\

P(+1 | \text{state is }|+\rangle )&=|| \Pi_{+1} |+\rangle ||^{2}= ||(|0\rangle \langle 0|)|+\rangle ||^2=|||0\rangle \langle 0|+\rangle ||^2
\end{align}

$$

We can expand out the norm squared here via $||\psi||^2=\psi\psi^*$ such that 

$$
\begin{align}
 P(+1 | \text{state is }|0\rangle )= \langle 0| \langle 0|0 \rangle |0\rangle \langle 0|0 \rangle =1
\end{align}
$$

and similarly

$$
P(+1 | \text{state is }|+\rangle ) =\langle 0| \langle +|0 \rangle |0 \rangle \langle 0|+ \rangle = \frac{1}{2}
$$

> [!help] Inner products
We note $\langle 0 | + \rangle = \langle+|0 \rangle =\frac{1}{\sqrt{ 2 }}$.

Hence, our final probability is 

$$
P(+1)=\frac{1}{4} \times 1+\frac{3}{4} \times \frac{1}{2}=\frac{5}{8}
$$

This is *incredibly long winded for a simple problem*. Whilst it is correct, there is a better way. 

Look at the above process, written in full here for convenience. 

$$
\begin{aligned}P(+1)&=P(\text{state is }|0\rangle)P(+1|\text{ state is }|0\rangle)+P(\text{state is }|+\rangle)P(+1|\text{ state is }|+\rangle)\\&=\frac{1}{4}\left\||(0\rangle\langle0|\right)|0\rangle\|^2+\frac{3}{4}||(0\rangle\langle0|)|+\rangle\|^2\\&=\frac{1}{4}\langle0|0\rangle\langle0|0\rangle+\frac{3}{4}\langle0|+\rangle\langle+|0\rangle\\&=\frac{5}{8}\end{aligned}
$$

We can rewrite the third line as 

$$
P(+1) = \langle 0| \left( \frac{1}{4}  |0\rangle \langle 0|+  \frac{3}{4} |+\rangle \langle +| \right) |0\rangle 
$$

The equation is interesting, because we have formed an operator inside that depends *only on the source*. This operator is known as the **density operator**, denoted by $\rho$.

$$
\rho= \frac{1}{4} |0\rangle \langle 0|+ \frac{3}{4}|+\rangle \langle + |
$$

With this in place, the probability to obtain the outcome +1 is simply

$$
P(+1) = \langle 0|\rho|0\rangle 
$$

which is a lot simpler. 

More generally, suppose the system emits systems in one of the $N$ states $|\psi_{n}\rangle$; $n \in \{1,2,\dots,N\}$, each with corresponding probability $p_{n}$ (we must have $\sum_{n}p_{n}=1$). The collection of these states, and associated probabilities $\{|\psi_{n}, p_{n}\}_{n}$ are referred to as an **ensemble of states**. 

> [!info] Definition of the density operator
> The density operator of this source is 
> $$\rho= \sum_{n} p_{n}|\psi_{n}\rangle \langle \psi_{n}|$$
> This is just the **average of the projectors** $|\psi_{n}\rangle \langle\psi_{n}|$ onto the states $|\psi_{n}\rangle$ emitted by the source. 

If we now consider measuring an arbitrary operator $A$ with eigenvalues and eigenstates $\lambda_{k}$ and $|e_{k}\rangle$ respectively, such that $A=\sum_{k}\lambda_{k}|e_{k}\rangle \langle e_{k}|$ we find

$$
P(\lambda_{k})= \sum_{n} P(\text{state is }|\psi_{n}\rangle ) \cdot P(\lambda_{k}|\text{state is}|\psi_{n})=\langle e_{k}|\rho|e_{k}\rangle 
$$

^be55cf

We can go further than this, but to do so, we need to introduce the **trace**.

> [!info] Definition of the trace
>
> The trace is a *linear operation* defined by the relation
> $$\text{tr}(|u\rangle \langle v|)=\langle v|u\rangle \qquad \text{for all }|u\rangle ,|v\rangle $$
> The fact that the trace is linear means that
> $$\text{tr}(\alpha |u\rangle \langle v| + \beta|w\rangle \langle x|)=\alpha \text{tr}(|u\rangle \langle v|)+\beta \text{tr}(|w\rangle \langle x|)$$
> for all $|u\rangle,|v\rangle,|w\rangle,|x\rangle$ and $\alpha, \beta \in \mathbb{C}$. 
> The trace can be thought of as moving the bra in front of the ket, then putting the together to form the inner product.

^fad126

We can use the trace to re-express 

$$
P(\lambda_{k})= \sum_{n} P(\text{state is }|\psi_{n}\rangle ) \cdot P(\lambda_{k}|\text{state is}|\psi_{n})=\langle e_{k}|\rho|e_{k}\rangle
$$

by noting that $\rho|e_{k}\rangle$ is a ket vector (just an operator acting on a ket). Using the definition of the trace, we can thus rewrite the above as 

$$
\langle e_{k}|\rho|e_{k}\rangle = \langle e_{k}|(\rho|e_{k}\rangle)=\text{tr}(|e_{k}\rangle (\langle e_{k}| \rho ))
$$

and hence 

$$
\text{Prob}(\lambda_{k})=\text{tr}(|e_{k}\rangle (\langle e_{k}| \rho )) = \text{tr}(\rho|e_{k}\rangle \langle e_{k}|)
$$

If we note that $\Pi_{k}$ is the projection operator associated with $|e_{k}\rangle$ then we can say that 

$$
\text{Prob}(\lambda_{k})=\text{tr}(\rho \Pi_{k})
$$

This is the simplest way to express the probability of the outcome of a measurement using the density operator formalism. 


