---
dg-publish: true
---
Given some operator $A$, its **adjoint $A^\dagger$** is given by

$$ \langle v| A^\dagger|w\rangle=\langle w|A|v\rangle^* $$

for _all vectors $|v\rangle$_ and _$|w\rangle$._


> [!Example]
> 
> Consider the operator $A$ in $\mathbb{C} ^2$ with matrix
> 
> $$ \begin{pmatrix} a & b \\ c & d \end{pmatrix} $$
> 
> It then follows that $A^\dagger$ will have matrix
> 
> $$ {\begin{pmatrix} a^* & c^* \\ b^* & d^* \end{pmatrix}}
> 
> $$
> ~={Grey}Take the transpose of the matrix and the the complex conjugate of all the values inside the matrix. =~



> [!Example]
> Let the operator $X$ have the matrix
> 
> $$ \begin{pmatrix} 0 & 1 \\ 1 & 0\end{pmatrix} $$
> 
> with respect to the standard basis. Then it follows that $X^\dagger$ will have the matrix
> 
> $$ \begin{pmatrix}0 & 1 \\ 1 & 0\end{pmatrix} $$
> 
> Since $X=X^\dagger$, we say that $X$ is **self-adjoint/hermitian**.
> 



$$ \big (|v\rangle\big )^\dagger=\langle v| $$

Recall that to a vector $|v\rangle$ we associated a _dual-vector $\langle v|$._ We can simply write

We can also note here that the dual vector to $A|v\rangle=\langle v|A$, where we have swapped the direction of operation. To see this, consider $\langle u|w\rangle=\langle w|u\rangle^*$. Let’s imagine that $A|v\rangle=|u\rangle$, such that

$$ \langle u|w\rangle=\langle w|A|v\rangle^*=\langle v|A^\dagger|w\rangle $$

This must be true for _all vectors $|w\rangle$_ as stated above, and so we can see that $\langle u|=\langle v|A^\dagger$.

It is a useful fact that $\big (|a\rangle\langle b|\big )^\dagger=|b\rangle\langle a|$. To see this, let $A=|a\rangle \langle b|$ and consider two arbitrary states $|v\rangle$ and $|w\rangle$. Then

$$ \begin{aligned}\langle v|A^\dagger|w\rangle &= \big( \langle w|A|v\rangle\big)^*\\ &=\big (\langle w|a\rangle\langle b|v\rangle\big)^* \quad \textcolor{oranglee}{\boxed{!}}\\ &= \langle a|w\rangle\langle v|b\rangle \\ &= \langle v|b\rangle\langle a|w\rangle \quad \\ &=\langle v| \big (|b\rangle\langle a| \big )|w\rangle\end{aligned}$$
~={Grey}Here we have skipped a step where we applied the complex conjugate to both inner products individually. This is essentially equivalent to multiplying through a bracket. Also note that inner products are scalars so their order of operation doesn’t matter. Hence we can swap them around in this step as so.=~

Since this is true for all $|v\rangle$ and $|w\rangle$, it must be the case that
$$
A^\dagger=\big (|a\rangle\langle b|\big )^\dagger=|b\rangle\langle a|
$$